add a bunch of primitives for BabyIPIngress WP proof

deps/poulet4/scratch/BabyIPIngress.v
@@ -7,6 +7,9 @@ Require Import Poulet4.Monads.Monad.
 Require Import Poulet4.Monads.State.
 Require Import Poulet4.Monads.Hoare.WP.
 
+From RecordUpdate Require Import RecordSet.
+Import RecordSetNotations.
+
 Open Scope string_scope.
 
 Import ListNotations.
@@ -206,12 +209,38 @@ Proof.
   intros. destruct vfi; auto.
 Qed.
 
+
+Lemma case_name_wp_p
+  {tags_t: Type}
+  {State Exception Result: Type}
+  {PBare PQualified}
+  {Q}
+  {cBare}
+  {cQualified: list (P4String.t tags_t) -> P4String.t tags_t -> @state_monad State Exception Result}
+  name :
+  (forall nm, name = BareName nm -> << PBare nm >> cBare nm << Q >>) ->
+  (forall nms nm, name = QualifiedName nms nm -> << PQualified nms nm >> cQualified nms nm << Q >>) ->
+  << 
+    match name with 
+    | BareName nm => PBare nm
+    | QualifiedName nms nm => PQualified nms nm 
+    end
+  >> 
+    match name with 
+    | BareName nm => cBare nm 
+    | QualifiedName nms nm => cQualified nms nm
+    end
+  << Q >>. 
+Proof.
+  destruct name; auto.
+Qed.
 Ltac wp' := 
   match goal with
   | [ |- << _ >> match ?e with | ValFuncImplBuiltin _ _ => _ | _ => _ end << _ >> ] => eapply (case_valfuncimpl_wp_p e)
   | [ |- << _ >> match ?e with | ValBase _ => _ | _ => _ end << _ >> ] => eapply (case_val_wp_p e)
   | [ |- << _ >> match ?e with | ValBaseNull => _ | _ => _ end << _ >> ] => eapply (case_valbase_wp_p e)
   | [ |- << _ >> match ?e with | ValObjTable _ => _ | _ => _ end << _ >> ] => eapply (case_valobj_wp_p e)
+  | [ |- << _ >> match ?e with | BareName _ => _ | _ => _ end << _ >> ] => eapply (case_name_wp_p e)
   end.
 
 Ltac wp_trans' := 
@@ -223,6 +252,296 @@ Definition eval_control (c: @Declaration Info) : env_monad Info unit :=
   | DeclControl _ nme tparams params cparams locals body => eval_block _ NoInfo body
   | _ => state_fail (AssertError "declaration is not a control")
   end.
+
+Instance etaEnvironment' {tags_t}: Settable _ := settable! MkEnvironment tags_t <(env_fresh _); (env_stack _); (env_heap _)>.
+
+
+Definition stack_pop_act {tags_t} (e: environment tags_t) : environment tags_t := 
+  match env_stack tags_t e with 
+  | nil => e
+  | _ :: es' => e <| env_stack _ := es' |>
+  end.
+
+Lemma stack_pop_wp_p
+  {tags_t: Type}
+  {Q} 
+  :
+  build_wp
+    (stack_pop tags_t)
+    (fun env => env_stack tags_t env <> nil)
+    Q
+    (fun env => (tt, stack_pop_act env )).
+Proof.
+  eapply build_wp_corr.
+  unfold stack_pop, stack_pop_act.
+  mysimp.
+  destruct env_stack; [exfalso; mysimp|].
+  simpl.
+  split; trivial.
+Qed.
+
+Lemma stack_push_wp_p
+  {tags_t: Type}
+  {Q} : 
+  build_wp
+    (stack_push tags_t)
+    top
+    Q
+    (fun (env: environment tags_t) => (tt, env <| env_stack _ := MStr.empty _ :: (env_stack _ env) |>)).
+Proof.
+  eapply build_wp_corr.
+  mysimp.
+Qed.
+
+(* some Props for reasoning about Environments, analogous to the MapsTo Prop for maps *)
+
+Require Import Coq.FSets.FMapList.
+Require Import Coq.Structures.OrderedTypeEx.
+Module Import MStr := Environment.MStr.
+
+Inductive Stack_MapsTo : string -> loc -> stack -> Prop :=
+  | InTopScope: 
+    forall str l top, MapsTo str l top -> 
+    forall stk, Stack_MapsTo str l (top :: stk)
+  | InInnerScope: 
+    forall str top,
+    (forall l, ~ MapsTo str l top) -> 
+    forall l' stk, Stack_MapsTo str l' stk -> 
+    Stack_MapsTo str l' (top :: stk)  
+  .
+
+Lemma stack_lookup'_l: 
+  forall str l stk, 
+    stack_lookup' str stk = Some l -> 
+    Stack_MapsTo str l stk.
+Proof.
+  intros.
+  induction stk; [exfalso; inversion H|].
+  (* destruct (find (elt:=l) str a). *)
+  admit.
+Admitted.
+
+(* not sure about this one; I'm positive it's true, but I'm not sure it's provable *)
+Lemma MapstoMissing: 
+  forall str mp,
+  (forall v : loc, ~ MapsTo str v mp) -> 
+  find str mp = None.
+Admitted.
+
+Lemma stack_lookup'_r: 
+  forall str l stk, 
+    Stack_MapsTo str l stk -> 
+    stack_lookup' str stk = Some l.
+Proof.
+  intros.
+  induction stk; inversion H; unfold stack_lookup'.
+  - erewrite find_1.
+    2: apply H3.
+    trivial.
+  - 
+    erewrite MapstoMissing; [|exact H4].
+    fold stack_lookup'.
+    auto.
+Qed.
+
+Lemma stack_lookup_wp_p
+  {tags_t}
+  {Q}
+  name loc: 
+  build_wp
+  (stack_lookup tags_t name)
+  (fun env => 
+    Stack_MapsTo name loc (env_stack tags_t env)
+  )
+  Q
+  (fun env => (loc, env)).
+Proof.
+  eapply build_wp_corr.
+  intros.
+  mysimp.
+  unfold stack_lookup.
+  rewrite (stack_lookup'_r name loc).
+  - mysimp.
+  - trivial.
+Qed.
+
+Module Import MNat := Environment.MNat.
+
+Inductive Heap_MapsTo {tags_t: Type} : loc -> @Value tags_t -> heap tags_t -> Prop :=
+  | MapsToInner : forall l v (hp: heap tags_t), MapsTo v l hp -> Heap_MapsTo v l hp.
+
+
+Lemma heap_lookup_wp_p
+  {tags_t}
+  {Q}
+  loc v: 
+  build_wp
+  (heap_lookup tags_t loc)
+  (fun env => 
+    Heap_MapsTo loc v (env_heap tags_t env)
+  )
+  Q
+  (fun env => (v, env)).
+Proof.
+  eapply build_wp_corr.
+  intros.
+  unfold hoare_partial_wp.
+  intros.
+  unfold heap_lookup.
+  destruct H. 
+  erewrite find_1.
+  2: { inversion H0; apply H1. }
+  simpl; split; trivial.
+Qed.
+
+Definition Env_MapsNameLoc 
+  {tags_t: Type}
+  (name: @Typed.name tags_t)
+  (l: loc)
+  (env: environment tags_t)
+  : Prop :=
+  match name with
+  | BareName nm => Stack_MapsTo (str nm) l (env_stack _ env)
+  | QualifiedName nil nm => 
+    match top_scope (env_stack _ env) with 
+    (* | Some st => Stack_MapsTo (str nm) l (st :: nil) *)
+    | Some st => False (* not supported for now *)
+    | None => False
+    end
+  | _ => False
+  end.
+
+Definition Env_MapsNameValue
+  {tags_t: Type}
+  (name: @Typed.name tags_t)
+  (l: loc)
+  (v: @Value tags_t)
+  (env: environment tags_t) 
+  : Prop := 
+    Env_MapsNameLoc name l env -> 
+    Heap_MapsTo l v (env_heap _ env).
+
+Definition eval_env_update 
+  {tags_t} 
+  (env: environment tags_t) 
+  (lv: @ValueLvalue tags_t) 
+  (v: @Value tags_t) 
+  : environment tags_t := 
+  match lv with 
+  | MkValueLvalue (ValLeftName (BareName nm) _) _ => 
+    match stack_lookup' (str nm) (env_stack _ env) with 
+    | Some l =>
+      env <| env_heap _ := Environment.MNat.add l v (env_heap _ env) |>
+    | None => env
+    end
+  | _ => env
+  end.
+
+Lemma get_name_loc_forward
+  {tags_t: Type}
+  l nm env: 
+  Env_MapsNameLoc nm l env ->
+  get_name_loc tags_t nm env = (inl l, env).
+Proof.
+  intros.
+  unfold Env_MapsNameLoc in H.
+  unfold get_name_loc.
+  destruct nm.
+  - unfold stack_lookup.
+    rewrite (stack_lookup'_r (str name) l (env_stack tags_t env)). 
+    + compute. trivial.
+    + trivial.
+  - destruct namespaces; [| exfalso; trivial].
+    simpl.
+    unfold state_bind, get_state.
+    unfold Transformers.lift_opt.
+    destruct (top_scope (env_stack tags_t env)); [| exfalso; trivial].
+    inversion H.
+Qed.
+
+Lemma heap_update_forward
+  {tags_t: Type}
+  l v v' env: 
+  Heap_MapsTo l v (env_heap tags_t env) -> 
+  let env' := (env <| env_heap _ := Environment.MNat.add l v' (env_heap _ env) |>) in 
+    heap_update _ l v' env = (inl tt, env').
+Proof.
+  intros.
+  inversion H.
+  unfold heap_update.
+  (* interestingly, our implementation of heap_update does not check for whether the address is in use or not *)
+  simpl.
+  unfold state_return.
+  trivial.
+Qed.
+
+
+
+Lemma get_name_loc_wp_p
+  {tags_t: Type}
+  {Q}
+  l nm: 
+  build_wp
+    (get_name_loc tags_t nm)
+    (fun env => Env_MapsNameLoc nm l env)
+    Q
+    (fun env => (l, env)).
+Proof.
+  eapply build_wp_corr.
+  mysimp.
+  unfold Env_MapsNameLoc in H0.
+
+  erewrite (get_name_loc_forward l).
+  - split; trivial.
+  - trivial.
+Qed.
+    
+Lemma env_update_wp_p 
+  {tags_t: Type}
+  {Q}
+  lv v:
+  build_wp
+    (env_update tags_t lv v)
+    (fun env => 
+      exists nm l v' locat ty, 
+        lv = MkValueLvalue (ValLeftName nm locat) ty /\
+        Env_MapsNameLoc nm l env /\
+        Env_MapsNameValue nm l v' env 
+    )
+    Q
+    (fun env => (tt, eval_env_update env lv v)). 
+Proof.
+  eapply build_wp_corr.
+  unfold hoare_partial_wp.
+  intros.
+  unfold env_update.
+  destruct H.
+  rewrite H in *.
+  clear H.
+  destruct H0 as [nm [l [v' [locat [ty H]]]]].
+  destruct H as [Hlv [Hn2l Hn2v]].
+  rewrite Hlv.
+
+  unfold mbind.
+  unfold state_monad_inst.
+  unfold state_bind.
+  erewrite (get_name_loc_forward l); [| trivial].
+
+
+  erewrite heap_update_forward.
+  - split; trivial.
+    unfold eval_env_update.
+    unfold Env_MapsNameLoc in Hn2l.
+    destruct nm.
+    + erewrite (stack_lookup'_r (str name) l); trivial.
+    + destruct namespaces; exfalso; trivial.
+      destruct (top_scope (env_stack tags_t st)); trivial.
+  - unfold Env_MapsNameValue in Hn2v.
+    apply Hn2v.
+    trivial.
+Qed.
+
+Require Import Poulet4.Unpack.
 
 Lemma baby_ip_ingress : 
   << top >>
@@ -253,61 +572,36 @@ Proof.
     unfold eval_packet_func;
     unfold Unpack.unpack_packet;
     wp_trans';
-    unfold mret, state_monad_inst; wp_trans'.
+    unfold mret, state_monad_inst, unpack_header; wp_trans'.
+
+
+  all: 
+    try (eapply stack_push_wp_p || 
+        eapply stack_pop_wp_p || 
+        eapply heap_lookup_wp_p || wp_trans').
+  all: unfold unpack_header, mret, state_monad_inst; wp_trans'.
+  4, 5: intros; eapply strengthen_pre_p; wp || app_ex.
+
+  12: {
+    unfold eval_cast.
+    Transparent mbind.
+    compute.
+    Opaque mbind.
+    app_ex.
+  }
+  10: {
+    unfold eval_cast.
+    Transparent mbind.
+    compute.
+    Opaque mbind.
+    app_ex.
+  }
+
+  10, 11: eapply env_update_wp_p.
 
     (* at this point, the primitives are 
-     * stack_pop, env_update, eval_cast, stack_push, stack_pop, eval_copy_out, 
-     * env_lookup, eval_push_front, eval_pop_front, env_update, unpack_header, 
-     * env_lookup, eval_copy_in, heap_lookup, stack_lookup 
+     * eval_copy_out, eval_copy_in,
+     * eval_push_front, eval_pop_front,
+     * and env_lookup.
      *)
 Admitted.
-
-
-(* some Props for reasoning about Environments, analogous to the MapsTo Prop for maps *)
-
-Require Import Coq.FSets.FMapList.
-Require Import Coq.Structures.OrderedTypeEx.
-Module Import MNat := Environment.MNat.
-Module Import MStr := Environment.MStr.
-
-Inductive Stack_MapsTo : string -> loc -> stack -> Prop :=
-  | InTopScope: 
-    forall str l top, MapsTo str l top -> 
-    forall stk, Stack_MapsTo str l (top :: stk)
-  | InInnerScope: 
-    forall str top,
-    (forall l, ~ MapsTo str l top) -> 
-    forall l' stk, Stack_MapsTo str l' stk -> 
-    Stack_MapsTo str l' (top :: stk)  
-  .
-
-Lemma stack_lookup'_l: 
-  forall str l stk, 
-    stack_lookup' str stk = Some l -> 
-    Stack_MapsTo str l stk.
-Proof.
-  intros.
-  induction stk; [exfalso; inversion H|].
-  (* destruct (find (elt:=l) str a). *)
-  admit.
-Admitted.
-
-Lemma stack_lookup'_r: 
-  forall str l stk, 
-    Stack_MapsTo str l stk -> 
-    stack_lookup' str stk = Some l.
-Proof.
-  intros.
-  induction stk; inversion H; unfold stack_lookup'.
-  - erewrite find_1.
-    2: apply H3.
-    trivial.
-  - 
-    assert ((forall loc0 : loc, ~ MapsTo str loc0 a) -> find str a = None).
-    admit.
-    specialize (H6 H4).
-    rewrite H6.
-    fold stack_lookup'.
-    auto.
-Admitted.
-
